i think the theorems are stated

Leanegraph/core/Naive.lean
@@ -1,68 +1,44 @@
 import Leanegraph.core.SharedDefs
-import Leanegraph.core.Helpers
-import Leanegraph.core.Hashcons
+import Leanegraph.core.ListAsMaps
+import Leanegraph.core.UnionFind
+import Leanegraph.core.NaiveDefs
 
 /-
-  Implementations of E-Node, E-Class, E-Graph and functions that operate on them
+  Naive.lean consists of most of the EGraph operations used in the
 -/
 variable {α : Type _} [DecidableEq α] [Hashable α] [Repr α]
 variable {D : Type _} [DecidableEq D] [Inhabited D]
 
 namespace Naive
 
-
-structure ENode (α : Type _ ) where
-  head : α
-  args : List EClassId
-deriving Hashable, DecidableEq, Repr
-
-structure EClass (α : Type _) (D : Type _) where
-  nodes : List (ENode α)
-  parents : List (ENode α × EClassId)
-  data : D
-deriving Repr
-
 /-
-  An e-graph is a tuple (U,M,H) of
-    Union-find U - Equivalence relation over *e-class ids*
-    E-class Map M - Map of *e-class ids to e-classes*
-    Hashcons H - Map of *e-nodes to e-class ids*
+  Define Helper Functions
 -/
+-- def ecmapLookup (eg : EGraph α D) : EClassId → Option (EClass α D) :=
+--  λ id => eg.ecmap.lookup id
+  -- eg.ecmap.lookup -- why doesn't this work? by some greek-letter-reduction
+  -- is it not the same thing?
 
-structure EGraph (α : Type _) (D : Type _) [DecidableEq α] [Hashable α] where
-  uf    : UF -- def UF := List <| EClassId × EClassId
-  ecmap : List <| EClassId × (EClass α D)
-  hcons : List <| ENode α × EClassId
-  dirty : List EClassId
-  aldrt : List EClassId
-/-
-def ufFind (eg : EGraph α D) (id : EClassId) : EClassId :=
-  eg.uf.lookup id |>.getD id
-
-def ufUnion (eg : EGraph α D)  (id₁ id₂ : EClassId) : EGraph α D :=
-  let leader₁ := ufFind eg id₁
-  let leader₂ := ufFind eg id₂
-  let newUf := eg.uf.map (λ (member, leader) =>
-    if leader == leader₂ then (member, leader₁) else (member, leader)
-  )
-  {eg with uf := newUf}
--/
-
-def ecmapLookup (eg : EGraph α D) : EClassId → Option (EClass α D) :=
-  λ id => eg.ecmap.lookup id
+def ecmapLookup (eg : EGraph α D) :=
+  eg.ecmap.lookup -- now it does with the new defs
 
 def hcLookup (eg : EGraph α D) : ENode α → Option EClassId :=
   λ en => eg.hcons.lookup en
 
 -- def insertHCons (hc : List <| ENode α × EClassId) (k : ENode α) (v : EClassId) : List <| ENode α × EClassId :=
---   (k, v) :: hc.filter (λ p => p.1 != k)
-def insertHCons (hc : List <| ENode α × EClassId) (k : ENode α) (v : EClassId) : List <| ENode α × EClassId :=
-  uniqueInsert hc k v
+--  uniqueInsert hc k v
 
-def insertECMap (ec : List <| EClassId × EClass α D) (k : EClassId) (v : EClass α D) : List <| EClassId × EClass α D :=
-  uniqueInsert ec k v
+def insertHCons (hc : ListMap (ENode α) EClassId): ENode α → EClassId → ListMap (ENode α) (EClassId) :=
+  λ k v => hc.insert k v
 
--- #eval List.filter (λ x => x ≠ 3) [1,2,3,4,5]
+def insertECMap (ec : ListMap EClassId (EClass α D)) (k : EClassId) (v : EClass α D) : ListMap EClassId (EClass α D) :=
+  ec.insert k v
+
+-- def insertECMap (ec : List <| EClassId × EClass α D) (k : EClassId) (v : EClass α D) : List <| EClassId × EClass α D :=
+--  uniqueInsert ec k v
+
+
+
 
 def EGraph.size (eg : EGraph α D) : Nat :=
   List.length eg.uf
@@ -72,52 +48,6 @@ def numCanonClasses (eg : EGraph α D) : Nat :=
 
 def numClasses (eg : EGraph α D) : Nat :=
   eg.uf.map Prod.snd |>.eraseDups |>.length
-/-
-theorem theTwoFunctionsAboveAreEqual (eg : EGraph α D) (h : UF.pairCanon eg.uf)
-  : numCanonClasses eg = numClasses eg := by
-  unfold numCanonClasses numClasses
-  unfold UF.pairCanon at h
-  simp[]
-  suffices h :
-    (eg.uf.filter (fun x => x.fst == x.snd)).map Prod.fst = (eg.uf.map Prod.snd).eraseDups
-    by
-      simp[Eq.symm h]
-
-  apply List.ext_getElem
-
-  sorry
--/
-
-instance [Inhabited α] : Inhabited (ENode α) where
-  default := {
-    head := default
-    args := []
-  }
-
-instance [Inhabited D] : Inhabited (EClass α D) where
-  default := {
-    nodes := []
-    parents := []
-    data := default
-  }
-
-class Analysis (α : Type _) (D : Type _)  [DecidableEq α][Hashable α] where
-  make : (en : ENode α) → List D → D
-  join : D → D → D
-  modify : EGraph α D → EClassId → EGraph α D
-
-instance : Inhabited (Analysis α Unit) where
-  default := {
-    make    _  _ := (),
-    join    _  _ := (),
-    modify  eg _ := eg
-  }
-
-instance : Analysis α Unit where
-  make _ _ := ()
-  join _ _ := ()
-  modify eg _ := eg
-
 
 /-
   Makes an instance of an EClass, either empty of from a Node
@@ -145,22 +75,52 @@ def EClass.merge [Analysis α D] (ec₁ ec₂ : EClass α D) : EClass α D:=
     data := Analysis.join (α := α) (D := D) (ec₁.data) (ec₂.data)
   }
 
+def EGraph.empty : EGraph α D:=
+  {
+    uf    := []
+    ecmap := ⟨[], by simp[KeysUnique]⟩
+    hcons := ⟨[], by simp[KeysUnique]⟩ -- ListMap.empty
+    dirty := []
+    aldrt := []
+  }
+
+
+
+
+/-
+  Update Parents in an E-Class. Two versions available, a fold and a map.
+  Maps seem to be easier to reason about, so use the map and do a performance check
+  to figure out which one to use for the optimised version
+  or think about the best way to do it
+  Calls:
+    - N/A
+  Called By:
+    - Push (en is canonicalised already, no need to canonicalise again)
+  Invariants:
+    - ?
+  Also it doesn't touch the Prod.fst which we have a lemma for (or can adapt)
+-/
+/-
 def updateEClassParents (en : ENode α) (eid : EClassId) (cur : EClassId × EClass α D) : EClassId × EClass α D :=
   (cur.1, ec) where
     parent := (en, eid)
     ec     := {cur.2 with parents := parent :: cur.2.parents}
-
-/-
-def updateParents (ecmap : List <| EClassId × EClass α D) (en : ENode α) (eid : EClassId)
-  : List <| EClassId × (EClass α D) :=
-  ecmap.map
-    (λ el@(id, _) =>
-      if id ∈ en.args then
-        updateEClassParents en eid el
-      else
-        el
-    )
 -/
+
+def updateEClassParents (en : ENode α) (eid : EClassId) (ec : EClass α D) : EClass α D :=
+  { ec with parents := (en, eid) :: ec.parents}
+
+
+def updateParents (ecmap : ListMap EClassId (EClass α D)) (en : ENode α) (eid : EClassId)
+  : ListMap EClassId (EClass α D) :=
+  ecmap.map
+    (λ id cls =>
+      if id ∈ en.args then
+        updateEClassParents en eid cls
+      else
+        cls
+    )
+/-
 def updateParents (ecmap : List <| EClassId × EClass α D) (en : ENode α) (eid : EClassId)
   : List <| EClassId × (EClass α D) :=
   en.args.foldl (λ acc argId =>
@@ -170,69 +130,44 @@ def updateParents (ecmap : List <| EClassId × EClass α D) (en : ENode α) (eid
         insertECMap acc argId updatedEc
     | none => acc
   ) ecmap
+-/
 
 
-def EGraph.empty : EGraph α D:=
-  {
-    uf    := []
-    ecmap := []
-    hcons := []
-    dirty := []
-    aldrt := []
-  }
 
-abbrev EGraphM (α : Type _) (D : Type _) [DecidableEq α] [Hashable α] := StateM (EGraph α D)
 /-
-def lookupCanonicalEClassId (id : EClassId) : EGraphM α D <| EClassId := do
-  let eg ← get
-  let ⟨uf', res⟩ := eg.uf.ufFind id
-  let _ ← set { eg with uf := uf' }
-  return res
+  lookupCanonicalEClassId:
+    - Finds the representative of the ECID in the UF
+  Calls: - N/A
+  Called By:
+    Repair(s), Rebuild, Union, Canonicalise
+  Notes: Seems to be overused in these functions, maybe cut down
 -/
 def lookupCanonicalEClassId (eg : EGraph α D) (id : EClassId) : EClassId :=
   eg.uf.find id
-/-
-def lookupCanonicalEClassIdM (id : EClassId) : EGraphM α D <| EClassId := do
-  let eg ← get
-  return eg.uf.find id
 
-def canonicaliseM (en : ENode α) : EGraphM α D (ENode α) := do
-  let newargs : List EClassId ← en.args.mapM lookupCanonicalEClassIdM
-  return { en with args := newargs}
+/-
+  Canonicalise:
+    - Canonicalises a node by replacing the arg ids with their canonical ids
+  Calls: lookupCanonicalEClassId
+  Called By: Push, Repair
 -/
 def canonicalise (eg : EGraph α D) (en : ENode α) : ENode α :=
   {en with args := en.args.map (lookupCanonicalEClassId eg)}
-/-
-def betterCanonicaliseM? (en : ENode α) : EGraphM α D (ENode α) := do
-  let eg ← get
-  return canonicalise eg en
--/
 
 
 /-
+  findClass:
+    - Lookup the E-Node in the HashCons
   Calls:
-    - Canonicalise
+    - N/A
   Called By:
     - Push (node canonicalised before call, no need to canon it again)
   Do we need to lookupCanonicalEClassId the hcons lookup?
-  In the naive, the hcons should always be canon
 -/
-def findClassM (en : ENode α) : EGraphM α D (Option EClassId) := do
-  -- let en' ← canonicalise en
-  let eg ← get
-  /-
-  match eg.hcons.lookup en with
-  | some eClassId =>
-    return some eClassId
-  | none =>
-    return none
-  -/
-  -- return eg.hcons.lookup en
-  return hcLookup eg en
+-- def findClass (eg : EGraph α D) (en : ENode α) : Option EClassId :=
+  -- hcLookup eg en
 
 
-def findClass (eg : EGraph α D) (en : ENode α) : Option EClassId :=
-  hcLookup eg en
 
 
 /-
@@ -240,9 +175,13 @@ def findClass (eg : EGraph α D) (en : ENode α) : Option EClassId :=
   If it exists, does nothing and returns ID
   If it doesn't, add it to the UF, E-Class Map, HCons
   Returns the new ID (which is the size of the E-Graph)
+
+  ecmapLookup takes canonical arguments
+  THINK:
+    hclookup uses a canonicalised en' as key
+    What is the state of the hashcons before this? -- can be anything, can't enforce anything
+    doesn't make hashcons stale, either adds a new node as new class or no-op
 -/
-
-
 def push [Analysis α D] (eg : EGraph α D) (en : ENode α) : EGraph α D × EClassId :=
   let en' := canonicalise eg en
   match hcLookup eg en' with
@@ -291,9 +230,9 @@ def union [Analysis α D] (eg : EGraph α D) (id₁ id₂ : EClassId) : EGraph �
     -- let ecmap'    := uniqueInsert (uniqueRemove eg.ecmap frId) leaderClassId newEClass
 
     -- Insert new leader class
-    let ecmap'    := uniqueInsert eg.ecmap leaderClassId newEClass
+    let ecmap'    := eg.ecmap.insert leaderClassId newEClass
     -- Replace old follower class with empty class for.... idk reasons (leave alone because I don't think deleting is good in array later)
-    let ecmap''   := uniqueInsert   ecmap' frId          EClass.empty
+    let ecmap''   := ecmap'.insert   frId          EClass.empty
 
     let newData   := newEClass.data
     let newDirty  := leaderClassId :: eg.dirty
@@ -313,8 +252,6 @@ def union [Analysis α D] (eg : EGraph α D) (id₁ id₂ : EClassId) : EGraph �
     }
 
     (Analysis.modify eg' leaderClassId, leaderClassId)
-
-def unionReduces : sorry := sorry
 
 
 def repairAnalysis [Analysis α D] (eg : EGraph α D) (id : EClassId) : EGraph α D :=
@@ -344,54 +281,59 @@ def repairAnalysis [Analysis α D] (eg : EGraph α D) (id : EClassId) : EGraph �
       Analysis.modify eg' canonId
     else eg
 
+def repairLoop1 (eg : EGraph α D) (eCls : EClass α D) : EGraph α D  × List (EClassId × EClassId) :=
+    let (updateHCons, collisions) := eCls.parents.foldl (init := (eg.hcons, [])) (λ (hcons', collisions') (node, pId) =>
+    let canonNode := canonicalise eg node
+    let canonId  := lookupCanonicalEClassId eg pId
+    let det      := hcons'.remove node --hcons'.filter (λ hc => hc.1 ≠ node)
+    match det.lookup canonNode with
+    | some key => (det, (canonId, key) :: collisions')
+    | none     => (det.insert canonNode canonId, collisions')
+    )
+  let eg' := {eg with hcons := updateHCons}
 
-def repair (eg : EGraph α D) (id : EClassId) : EGraph α D × List (EClassId × EClassId) :=
+  (eg', collisions)
+
+def repairLoop2 (eg : EGraph α D) (eCls : EClass α D) : EClass α D × List (EClassId × EClassId) :=
+  let (_, pc) := eCls.parents.foldl (init := ([], [])) (λ (seen, pc) (p : (ENode α × EClassId)) =>
+    let canon := canonicalise eg p.1
+    let canonId := lookupCanonicalEClassId eg p.2
+    match seen.lookup canon with
+    | some eid => (seen, (eid, canonId) :: pc)
+    | none     => ((canon, canonId) :: seen, pc)
+  )
+
+  let newNodes := eCls.nodes.foldl (init := []) (λ newN en =>
+    let canonN := canonicalise eg en -- or eg'?
+    -- if newN.any (λ a => a == canonN) then newN else canonN :: newN
+    if newN.contains canonN then newN else canonN :: newN
+  )
+
+  let newParents := eCls.parents.foldl (init := []) (λ newP (en, eid) =>
+    let canonN  := canonicalise eg en
+    let canonId := lookupCanonicalEClassId eg eid
+    if newP.any (λ (an, ac) => an == canonN && ac == canonId) then newP else (canonN, canonId) :: newP
+  )
+
+  ({nodes := newNodes, parents := newParents, data := eCls.data}, pc)
+
+
+def repair (eg : EGraph α D) (id : EClassId) : EGraph α D × (List <| EClassId × EClassId) :=
   let canonId := lookupCanonicalEClassId eg id
 
   match ecmapLookup eg canonId with
   | none => (eg, []) --
   | some eCls =>
 
-    let (updateHCons, collisions) := eCls.parents.foldl (init := (eg.hcons, [])) (λ (hcons', collisions') (node, pId) =>
-      let canonNode := canonicalise eg node
-      let canonId  := eg.uf.find pId
-      let det      := hcons'.filter (λ hc => hc.1 ≠ node)
-      match det.lookup canonNode with
-      | some key => (det, (canonId, key) :: collisions')
-      | none     => ((canonNode, canonId) :: det, collisions')
-    )
-
-    let eg' := {eg with hcons := updateHCons}
-
-
-
-
+    -- Hashcons Repair Loop
+    let (eg', collisions) := repairLoop1 eg eCls
 
     -- Loop 2...
-    let (_, pc) := eCls.parents.foldl (init := ([], [])) (λ (seen, pc) (p : (ENode α × EClassId)) =>
-      let canon := canonicalise eg' p.1
-      let canonId := lookupCanonicalEClassId eg' p.2
-      match seen.lookup canon with
-      | some eid => (seen, (eid, canonId) :: pc)
-      | none     => ((canon, canonId) :: seen, pc)
-    )
-
-    let newNodes := eCls.nodes.foldl (init := []) (λ newN en =>
-      let canonN := canonicalise eg' en -- or eg'?
-      -- if newN.any (λ a => a == canonN) then newN else canonN :: newN
-      if newN.contains canonN then newN else canonN :: newN
-    )
-
-    let newParents := eCls.parents.foldl (init := []) (λ newP (en, eid) =>
-      let canonN  := canonicalise eg' en
-      let canonId := lookupCanonicalEClassId eg eid
-      if newP.any (λ (an, ac) => an == canonN && ac == canonId) then newP else (canonN, canonId) :: newP
-    )
+    -- Repairs eClass
+    let (eCls', pc) := repairLoop2 eg' eCls
 
     let eg'' := { eg' with
-      ecmap := insertECMap eg'.ecmap canonId {eCls with
-        nodes := newNodes, parents := newParents
-      }
+      ecmap := insertECMap eg'.ecmap canonId eCls'
     }
 
     (eg'', collisions ++ pc)
@@ -402,30 +344,150 @@ def rebuildTerminationBy (eg : EGraph α D) : Nat × Nat :=
   let classes := numCanonClasses eg
   (classes, work)
 
-def rebuild [Analysis α D] (eg : EGraph α D) : EGraph α D :=
+
+def mergeCollisions [Analysis α D] (eg : EGraph α D) (collisions : List <| EClassId × EClassId)
+    : EGraph α D :=
+  collisions.foldl (λ acc (id₁, id₂) =>
+    (union acc id₁ id₂).1) eg
+
+def congruenceRepair [Analysis α D] (eg : EGraph α D) : EGraph α D :=
+  let todo := eg.dirty.map (lookupCanonicalEClassId eg) |>.eraseDups
+  let eg'  := {eg with dirty := []}
+
+  -- Pass through dirty (congruence repair)
+  -- extract the nested loop for readability
+  let eg'' := todo.foldl (λ eg₁ id =>
+    let (eg₂, collisions) := repair eg₁ id
+    mergeCollisions eg₂ collisions
+  ) eg'
+    /-
+    collisions.foldl (λ acc (id₁, id₂) =>
+      (union acc id₁ id₂).1) eg₂
+    ) eg'
+    -/
+
+  eg''
+
+def analysisRepair [Analysis α D] (eg : EGraph α D) : EGraph α D :=
+  -- Pass through aldrt (uh... analysis repair?)
+  let atodo := eg.aldrt.map (lookupCanonicalEClassId eg) |>.eraseDups
+  let eg'   := { eg with aldrt := [] }
+  let eg''   := atodo.foldl repairAnalysis eg'
+
+  eg''
+
+
+def singleRebuildPass [Analysis α D] (eg : EGraph α D) : EGraph α D :=
+  let eg' := congruenceRepair eg
+  let eg'':= analysisRepair eg'
+  eg''
+
+
+partial def rebuild [Analysis α D] (eg : EGraph α D) : EGraph α D :=
   if eg.dirty.isEmpty && eg.aldrt.isEmpty then eg
   else
-    let todo := eg.dirty.map (lookupCanonicalEClassId eg) |>.eraseDups
-    let eg'  := {eg with dirty := []}
+    let eg' := singleRebuildPass eg
+    rebuild eg'
 
-    -- Pass through dirty (congruence repair)
-    let eg'' := todo.foldl (λ eg₁ id =>
-      let (eg₂, collisions) := repair eg₁ id
-      collisions.foldl (λ acc (id₁, id₂) =>
-        (union acc id₁ id₂).1) eg₂
-      ) eg'
-    -- Pass through aldrt (uh... analysis repair?)
-    let atodo := eg''.aldrt.map (lookupCanonicalEClassId eg'') |>.eraseDups
-    let eg₃   := { eg'' with aldrt := [] }
-    let eg₄   := atodo.foldl repairAnalysis eg₃
 
-    rebuild eg₄
-termination_by (numClasses eg, eg.dirty.length + eg.aldrt.length)
+
+
+/-
+  Exports for outside use
+-/
+abbrev EGraphM (α : Type _) (D : Type _) [DecidableEq α] [Hashable α] := StateM (EGraph α D)
+
+def lookupCanonicalEClassIdM (id : EClassId) : EGraphM α D EClassId := do
+  return lookupCanonicalEClassId (← get) id
+
+def pushM [Analysis α D] (en : ENode α) : EGraphM α D EClassId := do
+  let (eg', id) := push (← get) en
+  discard <| set eg'
+  return id
+
+def unionM [Analysis α D] (id₁ id₂ : EClassId) : EGraphM α D EClassId := do
+  let (eg', leader) := union (← get) id₁ id₂
+  set eg'
+  return leader
+
+def rebuildM [Analysis α D] : EGraphM α D Unit := do
+  set (rebuild (← get))
+
+
+
+
+
+
+
+
+
+
+
+
+
+
+
+
+
+
+
+
+
+
+
+
+
+
+
+/-
+def lookupCanonicalEClassId (id : EClassId) : EGraphM α D <| EClassId := do
+  let eg ← get
+  let ⟨uf', res⟩ := eg.uf.ufFind id
+  let _ ← set { eg with uf := uf' }
+  return res
+-/
+/-
+def lookupCanonicalEClassIdM (id : EClassId) : EGraphM α D <| EClassId := do
+  let eg ← get
+  return eg.uf.find id
+
+def canonicaliseM (en : ENode α) : EGraphM α D (ENode α) := do
+  let newargs : List EClassId ← en.args.mapM lookupCanonicalEClassIdM
+  return { en with args := newargs}
+-/
+/-
+def betterCanonicaliseM? (en : ENode α) : EGraphM α D (ENode α) := do
+  let eg ← get
+  return canonicalise eg en
+-/
+
+
+/-
+def findClassM (en : ENode α) : EGraphM α D (Option EClassId) := do
+  -- let en' ← canonicalise en
+  let eg ← get
+  /-
+  match eg.hcons.lookup en with
+  | some eClassId =>
+    return some eClassId
+  | none =>
+    return none
+  -/
+  -- return eg.hcons.lookup en
+  return hcLookup eg en
+-/
+
+
+
+/-
+termination_by rebuildTerminationBy eg -- (numClasses eg, eg.dirty.length + eg.aldrt.length)
 decreasing_by
   simp_wf
-
+  cases
+  case pos => sorry
+  case neg => sorry
   sorry
-
+-/
 -- https://leanprover-community.github.io/extras/well_founded_recursion.html
 -- Bottom of the page has example on Nat × Nat
 
@@ -457,29 +519,6 @@ def unionRun [Analysis α D] (id₁ id₂ : EClassId) : EGraphM α D EClassId :=
 /-
   Props that might be needed eventually?
 -/
-
-
-
-
-/-
-  Exports for outside use
--/
-
-def lookupCanonicalEClassIdM (id : EClassId) : EGraphM α D EClassId := do
-  return lookupCanonicalEClassId (← get) id
-
-def pushM [Analysis α D] (en : ENode α) : EGraphM α D EClassId := do
-  let (eg', id) := push (← get) en
-  discard <| set eg'
-  return id
-
-def unionM [Analysis α D] (id₁ id₂ : EClassId) : EGraphM α D EClassId := do
-  let (eg', leader) := union (← get) id₁ id₂
-  set eg'
-  return leader
-
-def rebuildM [Analysis α D] : EGraphM α D Unit := do
-  set (rebuild (← get))
 
 
 
