Leanegraph/core/Invariants.lean
@@ -1,0 +1,202 @@
+import Leanegraph.core.UnionFind
+import Leanegraph.core.ListAsMaps
+import Leanegraph.core.Naive
+import Leanegraph.core.NaiveDefs
+import Leanegraph.core.SharedDefs
+
+variable {α : Type _} [DecidableEq α] [Hashable α] [Repr α]
+variable {D : Type _} [DecidableEq D] [Inhabited D]
+
+namespace Naive
+
+/-
+  Props of E-Nodes
+-/
+-- An ENode is canonical if all arguments are canonical
+def ENode.isCanonical (en : ENode α) (eg : EGraph α D) : Prop :=
+  ∀ arg ∈ en.args, arg = lookupCanonicalEClassId eg arg
+  -- en.args.map (lookupCanonicalEClassId eg) = en.args
+  -- should be the same, figure out which one is better
+
+-- Two ENodes are congruent if head is equal, all args are in same eclass
+def ENode.isCongruent (en₁ en₂ : ENode α) (eg : EGraph α D) : Prop :=
+-- Is there a zip in lean?
+-- https://leanprover-community.github.io/mathlib4_docs/Mathlib/Data/List/Forall2.html This is pretty cool
+-- Oh it's mathlib
+-- Back to zip
+  -- en₁.head = en₂.head ∧ (en₁.args.zip en₂.args).all (λ (a, b) ↦ lookupCanonicalEClassId a = lookupCanonicalEClassId b)
+  en₁.head = en₂.head ∧
+  en₁.args.length = en₂.args.length ∧
+  (en₁.args.zip en₂.args).all (λ (a, b) ↦ lookupCanonicalEClassId eg a = lookupCanonicalEClassId eg b)
+
+
+
+-- EGraph Components
+-- ecmap, hcons always unique keys if the functions defined in ListAsMaps.lean are used
+
+
+/-
+  Props about the EGraph State
+-/
+def EGraph.isClean (eg : EGraph α D) : Prop :=
+  eg.dirty.isEmpty ∧ eg.aldrt.isEmpty
+
+/-
+  That the dirty and aldrt (analysis dirty) lists hold only valid IDs
+-/
+def EGraph.dirtyValid (eg : EGraph α D) : Prop :=
+  ∀ id ∈ eg.dirty, eg.uf.isValidID id
+
+def EGraph.aldrtValid (eg : EGraph α D) : Prop :=
+  ∀ id ∈ eg.aldrt, eg.uf.isValidID id
+
+
+-- Hashcons is correct when all enodes in it are canonical and the enodes point to a canonical id
+-- Hashcons can be stale, between union and rebuild
+def hashconsCanonical (eg : EGraph α D) : Prop :=
+  ∀ en id, eg.hcons.lookup en = some id → en.isCanonical eg ∧ lookupCanonicalEClassId eg id = id
+
+
+-- every valid entry in hcons is valid in the ecmap (when canon id)
+-- does this hold between union and rebuild
+-- connects the 3 parts of the egr
+def EGraph.hconsToEcmap (eg : EGraph α D) : Prop :=
+  ∀ en id, hcLookup eg en = some id →
+    ∃ cls, ecmapLookup eg (lookupCanonicalEClassId eg id) = some cls
+
+/-
+  Define the two main invariants for E-Graphs.
+  1. Congruence Invariant
+    The e-graph must ensure that congruent e-nodes are in the same e-class
+
+  2. Hashcons Invariant
+    From Egg: e-node 𝑛∈𝑀[𝑎] ⇐⇒ 𝐻[canonicalize(𝑛)]=find(𝑎)
+    The hashcons 𝐻 must map all canonical e-nodes to their e-class ids
+    enode en is in eclass (ecmap id₁) IFF hashcons.lookup(en) = uf.find id
+
+  Bonus: Some analysis invariant?
+    ∀𝑐∈𝐺. 𝑑𝑐=Ûmake(𝑛) and modify(𝑐)=𝑐 (copied egg pg.13, idk how to type that, TODO: )
+-/
+def EGraph.congruenceInvariant
+    -- (eg : EGraph α D) (en₁ en₂ : ENode α) (id₁ id₂ : EClassId) : Prop := -- no need to specify
+    (eg : EGraph α D) : Prop :=
+      ∀ en₁ en₂ id₁ id₂, -- forall en/id ₁₂ where
+        eg.hcons.lookup en₁ = some id₁ → -- id₁ is the canon class of en₁
+        eg.hcons.lookup en₂ = some id₂ → -- and id₂ of en₂
+        ENode.isCongruent en₁ en₂ eg →  -- and the two nodes are congruent
+        lookupCanonicalEClassId eg id₁ = lookupCanonicalEClassId eg id₂ -- the two nodes are in the same e-class
+
+
+def inEClass (eg : EGraph α D) (en : ENode α) (id : EClassId) : Prop :=
+  ∃ ecls, ecmapLookup eg id = some ecls ∧ en ∈ ecls.nodes
+
+def EGraph.hashconsInvariant (eg : EGraph α D) : Prop :=
+  ∀ (en : ENode α) (id : EClassId),
+    -- e-node 𝑛∈𝑀[𝑎]
+    inEClass eg en id
+    ↔
+    -- 𝐻[canonicalize(𝑛)]=find(𝑎)
+    hcLookup eg (canonicalise eg en) = lookupCanonicalEClassId eg id
+-- huh doesn't this imply the congruenceInvariant? In the ← direction?
+-- TODO: go for this one first, I think?
+
+
+-- Invariants that must always hold
+def EGraph.alwaysInvariants (eg : EGraph α D) : Prop :=
+  UF.wellFormed eg.uf ∧ -- all IDs are valid and is flat
+  -- ecmap/hcons has unique keys, but that is from subtype, not mentioned here
+  -- still keep that in mind, probably need
+  eg.dirtyValid ∧
+  eg.aldrtValid ∧
+  eg.hconsToEcmap
+  -- i think this is about it?
+  -- hcons can go stale, ecmap can go stale
+  -- uf is i think always valid?
+
+theorem pushPreservesAlwaysInvariants [Analysis α D] (eg : EGraph α D)
+  (h : eg.alwaysInvariants) (en : ENode α) :
+    (push eg en).1.alwaysInvariants := by
+  sorry
+
+theorem unionPreservesAlwaysInvariants [Analysis α D] (eg : EGraph α D)
+  (h : eg.alwaysInvariants) (id₁ id₂ : EClassId) :
+    (union eg id₁ id₂).1.alwaysInvariants := by
+  sorry
+
+theorem repairPreservesAlwaysInvariants [Analysis α D] (eg : EGraph α D)
+  (h : eg.alwaysInvariants) (id : EClassId) :
+    (repair eg id).1.alwaysInvariants := by
+  sorry
+
+theorem rebuildPreservesAlwaysInvariants [Analysis α D] (eg : EGraph α D)
+  (h : eg.alwaysInvariants) (id : EClassId) :
+    (singleRebuildPass eg).alwaysInvariants := by
+  sorry
+
+
+
+-- Invariants that are repaired by the rebuild process
+def EGraph.afterRebuildInvariants (eg : EGraph α D) : Prop :=
+  eg.alwaysInvariants ∧ eg.hashconsInvariant ∧ eg.congruenceInvariant ∧ eg.isClean
+-- if hashconsInv → congruenceInv then this only needs to mention 3?
+
+theorem rebuildRestoresInvariants [Analysis α D] (eg : EGraph α D)
+    (h : eg.alwaysInvariants) : (rebuild eg).afterRebuildInvariants := by
+  sorry
+
+
+/-
+theorem twoNodesInSameEClassMustBeCongruent [Analysis α D] (eg : EGraph α D)
+    (h : eg.afterRebuildInvariants) (id₁ id₂ : EClassId) (en₁ en₂ : ENode α) :
+
+  sorry
+-/
+
+
+-- Talk about the newly extracted mini-functions of repair and rebuild
+theorem repairLoop1NoTouchUF (eg : EGraph α D) (eCls : EClass α D) :
+    (repairLoop1 eg eCls).1.uf = eg.uf := by
+  sorry
+
+theorem repairLoop1HConsRepaired (eg : EGraph α D) (eCls : EClass α D) :
+    ∀ (id₁ id₂ : EClassId), (id₁, id₂) ∈ (repairLoop1 eg eCls).2 →
+      ∃ en, hcLookup eg en = some id₁ ∨ hcLookup eg en = some id₂ := by
+  sorry
+
+
+-- theorem repairLoop2UpdatesEClassOnly (eg : EGraph α D) (eCls : EClass α D) :
+-- also a NoTouchUF, but also NoTouchHCons/ECMap/Anything
+-- This doesn't touch eg
+-- Doesn't even return an eg. What now?
+--   (repairLoop2 eg eCls)
+
+theorem mergeCollisionsPreservesAlwaysInvariants [Analysis α D] (eg : EGraph α D)
+    (h : eg.alwaysInvariants) (collisions : List (EClassId × EClassId)) :
+      (mergeCollisions eg collisions).alwaysInvariants := by
+  sorry
+
+theorem congruenceRepairPreservesAlwaysInvariants [Analysis α D] (eg : EGraph α D) (h : eg.alwaysInvariants) :
+    (congruenceRepair eg).alwaysInvariants := by
+  sorry
+
+theorem analysisRepairPreservesAlwaysInvariants [Analysis α D] (eg : EGraph α D) (h : eg.alwaysInvariants) :
+    (analysisRepair eg).alwaysInvariants := by
+  sorry
+
+theorem singleRebuildPassPreservesAlwaysInvariants [Analysis α D] (eg : EGraph α D) (h : eg.alwaysInvariants) :
+    (singleRebuildPass eg).alwaysInvariants := by
+  simp[singleRebuildPass]
+  apply analysisRepairPreservesAlwaysInvariants
+  apply congruenceRepairPreservesAlwaysInvariants
+  apply h
+
+
+-- Ultimate Theorem?
+theorem egraphCorrect [Analysis α D] (eg : EGraph α D)
+    (h : eg.afterRebuildInvariants) (en₁ en₂ : ENode α) (id₁ id₂ : EClassId)
+      (h₁ : inEClass eg en₁ id₁) (h₂ : inEClass eg en₂ id₂) :
+      -- two nodes are congruent iff same class
+        eg.uf.find id₁ = eg.uf.find id₂ ↔ ENode.isCongruent en₁ en₂ eg := by
+  sorry
+
+end Naive
