Leanegraph/core/ListAsMaps.lean
@@ -1,0 +1,348 @@
+variable {α β : Type _} [DecidableEq α]
+
+-- Inserts a key/value pair into the map
+-- Overwrites existing key
+-- TODO: do we ever need to reject existing keys?
+-- TODO: what did I mean by that?
+def uniqueInsert (cur : List (α × β)) (k : α) (v : β) : List <| α × β :=
+  (k, v) :: cur.filter (λ p => p.1 != k)
+
+-- Removes a key/value pair from the map.
+def uniqueRemove (cur : List (α × β)) (k : α) : List <| α × β :=
+  cur.filter (λ p => p.1 != k)
+
+def uniqueReplace : List (α × β) → α → β → List (α × β)
+| [],               _, _ => []
+| ((k', v') :: xs), k, v => if k == k' then (k, v) :: xs else (k', v') :: uniqueReplace xs k v
+
+
+-- this doesn't need the unique name but for the sake of consistency
+-- kinda interesting that the std impl. uses ```match k = k with true/false```,
+-- TODO: SOMEDAY: look that up one day
+-- better for simp? case splitting?
+-- iig can just use the standard and no need to define this
+/-
+def uniqueLookup : List (α × β) → α → Option β
+| [], _ => none
+| ((k', v) :: xs), k =>
+  if k = k' then some v else uniqueLookup xs k
+
+-- #eval uniqueLookup [(0,1), (2,4), (3,6)] 4
+-/
+/-
+not equal!! Replace must R E P L A C E and not I N S E R T
+def uniqueReplace' : List (α × β) → α → β → List (α × β) :=
+  λ cur k v => uniqueInsert (uniqueRemove cur k) k v
+-/
+
+def KeysUnique (cur : List (α × β)) : Prop :=
+  List.Nodup (cur.map Prod.fst)
+
+theorem keysUnique_filter
+  (xs : List (α × β)) (h : KeysUnique xs) (k : α) : KeysUnique (xs.filter (λ p => p.1 != k)) := by
+  induction xs with
+  | nil => simp[h]
+  | cons x xs ih =>
+    rcases List.nodup_cons.mp h with ⟨hx, hxs⟩
+    simp[KeysUnique, List.filter]
+    match h' : x.fst != k with
+    | true =>
+      apply List.nodup_cons.mpr
+      constructor
+      · intro hmem
+        rw [List.mem_map] at hmem
+        rcases hmem with ⟨p, hp1, hp2⟩
+        apply hx
+        rw[List.mem_map]
+        exact ⟨p, (List.mem_filter.mp hp1).1, hp2⟩
+      · rw[←KeysUnique] at hxs
+        rw[←KeysUnique]
+        exact ih hxs
+    | false =>
+      rw[←KeysUnique] at hxs
+      rw[←KeysUnique]
+      exact ih hxs
+
+
+
+theorem uniqueInsert_Preserves_Unique
+  (cur : List (α × β)) (hBefore : KeysUnique cur) (k : α) (v : β) : KeysUnique (uniqueInsert cur k v) :=
+  by
+    unfold KeysUnique
+    unfold uniqueInsert
+    apply List.nodup_cons.mpr
+    constructor
+    · intro hmem
+      rw [List.mem_map] at hmem
+      rcases hmem with ⟨p, hp, hpkey⟩
+      have hp' := List.mem_filter.mp hp
+      have hneq : p.1 != k := hp'.2
+
+      subst hpkey
+      simp[] at hneq
+    ·
+      rw [←KeysUnique]
+      exact keysUnique_filter cur hBefore k
+
+theorem uniqueRemove_Preserves_Unique
+  (cur : List (α × β)) (hBefore : KeysUnique cur) (k : α) : KeysUnique (uniqueRemove cur k) := by
+  exact keysUnique_filter cur hBefore k
+
+
+
+/-
+theorem uniqueReplace_Preserves_Unique
+  (cur : List (α × β)) (hBefore : KeysUnique cur) (k : α) (v : β) : KeysUnique (uniqueReplace cur k v) := by
+  unfold KeysUnique uniqueReplace
+  simp
+  induction cur with
+  | nil => simp[]
+  | cons x xs h =>
+    simp[]
+    split
+    case isTrue hEq =>
+      have hN : List.Nodup (k :: xs.map Prod.fst) := by
+        simpa [hEq, KeysUnique] using hBefore
+      simp[hN]
+    case isFalse hFalse =>
+      have hBefore' : List.Nodup (x.1 :: xs.map Prod.fst) := by
+        simpa [KeysUnique] using hBefore
+      rcases List.nodup_cons.mp hBefore' with ⟨hx, hxs⟩
+      constructor
+      ·
+
+      sorry
+-/
+
+
+theorem uniqueReplace_map_fst
+    (cur : List (α × β)) (k : α) (v : β) :
+    (uniqueReplace cur k v).map Prod.fst = cur.map Prod.fst := by
+  induction cur with
+  | nil =>
+      simp [uniqueReplace]
+  | cons x xs ih =>
+      simp [uniqueReplace]
+      split
+      · simp[]
+        assumption
+      · simp [ih]
+
+theorem uniqueReplace_Preserves_Unique
+  (cur : List (α × β))
+  (hBefore : KeysUnique cur)
+  (k : α)
+  (v : β) :
+  KeysUnique (uniqueReplace cur k v) := by
+  unfold KeysUnique
+  rw [uniqueReplace_map_fst]
+  exact hBefore
+
+
+/-
+  Instead of structure, apparently these subtype things are useful
+-/
+
+abbrev ListMap α β := { val : List (α × β) // KeysUnique val }
+
+def ListMap.empty : ListMap α β :=
+  ⟨
+    [],
+    by unfold KeysUnique; simp
+  ⟩
+
+
+def ListMap.insert (k : α) (v : β) (map : ListMap α β) : ListMap α β :=
+  ⟨
+    uniqueInsert map.val k v,
+    uniqueInsert_Preserves_Unique map.val map.2 k v
+  ⟩
+
+def ListMap.remove (k : α) (map : ListMap α β) : ListMap α β :=
+  ⟨
+    map.val.filter (λ p => p.1 != k),
+    keysUnique_filter map.val map.property k
+  ⟩
+
+
+def ListMap.replace (k : α) (v : β) (map : ListMap α β) : ListMap α β :=
+  ⟨
+    uniqueReplace map.val k v,
+    by
+      unfold KeysUnique
+      rw[uniqueReplace_map_fst]
+      exact map.property
+  ⟩
+
+def ListMap.lookup (map : ListMap α β) (k : α) : Option β :=
+  map.val.lookup k
+
+/-
+theorem mapNoTouchKeys {α β γ : Type _} (xs : List (α × β)) (f : β → γ) :
+      (xs.map (fun (k, v) => (k, f v))).map Prod.fst = xs.map Prod.fst := by
+  simp
+-/
+
+
+-- maybe i shouldn't call it map
+def ListMap.map {γ : Type _} (xs : ListMap α β) (f : α → β → γ) : ListMap α γ :=
+  ⟨
+    xs.val.map (λ (k, v) => (k, f k v)),
+    by
+      /-
+        Idea: Map doesn't touch keys, so KeysUnique is trivially preserved
+        H e l p e r  L e m m a
+        Maybe we can inline the helper lemma for brevity
+        Do we need the theorem separately..?
+        TODO:don't delete for later use (uncomment) if needed
+      -/
+      have mapNoTouchKeys (xs : List (α × β)) (f : β → γ) :
+        (xs.map (fun (k, v) => (k, f v))).map Prod.fst = xs.map Prod.fst := by
+        simp
+      unfold KeysUnique
+      simp -- [mapNoTouchKeys xs.val f]
+      -- SOMEDAY: lookup simp, does it try run things from context?
+      exact xs.property
+
+  ⟩
+
+
+-- Should this be a prop?
+def ListMap.contains (map : ListMap α β) (k : α) : Bool :=
+  map.val.any (λ (k', _) => k == k')
+
+def ListMap.notContains (map : ListMap α β) (k : α) : Prop :=
+  map.val.all (λ (k', _) => k != k')
+
+
+
+
+
+
+
+
+
+
+
+/-
+  Question: Can we encode the invariant into the type? That's a benefit of DTT right
+  A well formed map is one with unique keys, but how to encode?
+-/
+
+structure ListMapStr (α : Type _) (β : Type _) where
+  Vals   : List (α × β)
+  Unique : KeysUnique Vals -- reused
+
+-- #print ListMap -- structures are types, is this good enough?
+
+/-
+  Define our Insert, Replace, Delete Functions
+  For insert presumably induction is easiest,
+  define the base case
+-/
+
+-- Base Case is the existence of a well formed ListMap
+def emptyListMap : ListMapStr α β := ⟨[], by simp[KeysUnique]⟩
+
+/-
+  Proof Sketch:
+    - Given: Map is well formed (because it exists, yay!)
+    - Show:
+      - k ∉ map.Vals.filter
+      - Insert k is fine
+-/
+def ToListMap (k : α) (v : β) (map : ListMapStr α β) : ListMapStr α β :=
+  ⟨
+    (k, v) :: map.Vals.filter (λ p => p.1 != k),
+    by
+      unfold KeysUnique
+      apply List.nodup_cons.mpr -- break down nodup into its precond
+      /-
+        Goal at this point
+        ¬(k, v).fst ∈ List.map Prod.fst (List.filter (fun p => p.fst != k) map.Vals)
+        ∧
+        (List.map Prod.fst (List.filter (fun p => p.fst != k) map.Vals)).Nodup
+
+        Use constructor to break into the two halves
+      -/
+      constructor
+      · -- ¬(k, v).fst ∈ List.map Prod.fst (List.filter (fun p => p.fst != k) map.Vals)
+        -- In English: Show that k is not in the filtered list
+        intro hmem -- goal into "isMem → False"
+        -- Rewrite hmem
+        rw[List.mem_map] at hmem
+        rcases hmem with ⟨p, hp, hpkey⟩ -- break into parts
+        -- rcases can break down a fancy term into constituent parts in one go
+        rw[List.mem_filter] at hp -- rewrite the filter in hp
+        rcases hp with ⟨hp', hpNotkey⟩ -- hp broken into parts
+        simp at hpkey -- get "p.fst = k"
+        /-
+          Current State, we have
+            hpNotkey : (p.fst != k) = true and hpkey : p.fst = k (badly named)
+            Together we get a contradiction for prove goal of false
+        -/
+        rw[hpkey] at hpNotkey
+        simp at hpNotkey
+
+      · -- (List.map Prod.fst (List.filter (fun p => p.fst != k) map.Vals)).Nodup
+        -- In English: Show that the filtered list is nodup
+        rw[←KeysUnique]
+        -- Goal: KeysUnique (List.filter (fun p => p.fst != k) map.Vals)
+        apply keysUnique_filter map.Vals map.Unique
+  ⟩
+
+def ListMapStr.insert (k : α) (v : β) (map : ListMapStr α β) : ListMapStr α β :=
+  ⟨
+    (k, v) :: map.Vals.filter (λ p => p.1 != k),
+    by
+      unfold KeysUnique
+      apply List.nodup_cons.mpr
+      constructor
+      ·
+        intro hmem
+        rw[List.mem_map] at hmem
+        rcases hmem with ⟨p, hp, hpkey⟩
+        have hp' := List.mem_filter.mp hp
+        have hnm := hp'.2
+        subst hpkey
+        simp at hnm
+      ·
+        rw[←KeysUnique]
+        apply keysUnique_filter map.Vals map.Unique
+  ⟩
+
+
+/-
+  Since keys are unique, filtering by a key should do at most 1 pair of damage
+-/
+def ListMapStr.remove (k : α) (map : ListMapStr α β) : ListMapStr α β :=
+  ⟨
+    map.Vals.filter (λ p => p.1 != k),
+    by
+      exact keysUnique_filter map.Vals map.Unique k
+  ⟩
+
+theorem uniqueReplace_map_fst2
+    (cur : List (α × β)) (k : α) (v : β) :
+    (uniqueReplace cur k v).map Prod.fst = cur.map Prod.fst := by
+  induction cur with
+  | nil =>
+    rfl
+  | cons x xs ih =>
+    simp[uniqueReplace]
+    split
+    case isTrue =>
+      simpa -- simp + assumption?
+      -- assumption
+    case isFalse =>
+      simp[ih]
+
+
+def ListMapStr.replace (k : α) (v : β) (map : ListMapStr α β) : ListMapStr α β :=
+  ⟨
+    uniqueReplace map.Vals k v,
+    by
+      unfold KeysUnique
+      rw[uniqueReplace_map_fst2]
+      exact map.Unique
+  ⟩
