Leanegraph/core/NaiveDefs.lean
@@ -1,0 +1,105 @@
+import Leanegraph.core.SharedDefs
+import Leanegraph.core.UnionFind
+import Leanegraph.core.ListAsMaps
+
+variable {α : Type _} [DecidableEq α] [Hashable α] [Repr α]
+variable {D : Type _} [DecidableEq D] [Inhabited D]
+
+
+/-
+  In this file we define the basic structures: ENode, EClass, EGraph.
+  We also provide the class definition for Analysis
+    (TODO: why is this a class? does it matter? why?)
+
+  and the default inhabited instances for each of the structures
+-/
+
+namespace Naive
+
+structure ENode (α : Type _ ) where
+  head : α
+  args : List EClassId
+deriving Hashable, DecidableEq, Repr
+
+/-
+  The parents list is a list of ENodes and their (TODO: canonical? only after repair) IDs
+-/
+structure EClass (α : Type _) (D : Type _) where
+  nodes : List (ENode α)
+  parents : List (ENode α × EClassId)
+  data : D
+deriving Repr
+
+/-
+  An e-graph is a tuple (U,M,H) of
+    Union-find U - Equivalence relation over *e-class ids*
+    E-class Map M - Map of *e-class ids to e-classes*
+    Hashcons H - Map of *e-nodes to e-class ids*
+
+  In the naïve version, we model a map by a list
+  Helpers.lean defines operations and theorems that preserve map-like properties
+  Operations on the "maps" should use the defined wrappers and not the built in list ops
+-/
+structure EGraph (α : Type _) (D : Type _) [DecidableEq α] [Hashable α] where
+  uf    : UF -- def UF := List <| EClassId × EClassId
+  ecmap : ListMap EClassId (EClass α D) -- List <| EClassId × (EClass α D)
+  hcons : ListMap (ENode α) EClassId-- List <| ENode α × EClassId
+  dirty : List EClassId
+  aldrt : List EClassId
+
+/-
+  Analysis
+-/
+
+class Analysis (α : Type _) (D : Type _) [DecidableEq α] [Hashable α] where
+  make : (en : ENode α) → List D → D
+  join : D → D → D
+  modify : EGraph α D → EClassId → EGraph α D
+
+
+
+/---
+  -
+ ---/
+
+
+
+/-
+  Default Instances
+-/
+
+-- ENode
+instance [Inhabited α] : Inhabited (ENode α) where
+  default := {
+    head := default
+    args := []
+  }
+
+-- EClass
+instance [Inhabited D] : Inhabited (EClass α D) where
+  default := {
+    nodes := []
+    parents := []
+    data := default
+  }
+
+-- Analysis
+instance : Inhabited (Analysis α Unit) where
+  default := {
+    make    _  _ := (),
+    join    _  _ := (),
+    modify  eg _ := eg
+  }
+
+-- Analysis₂
+-- To be honest I cannot remember why we needed two
+-- TODO: figure this out I guess
+-- This one is not an Inhabited instance?
+instance : Analysis α Unit where
+  make _ _ := ()
+  join _ _ := ()
+  modify eg _ := eg
+
+
+
+end Naive
